

# Contents

<b>1</b>	<b>Integrals: Evil</b>	<b>2</b>
1.1	<u>Problem One</u> . . . . .	2
	1.1.1 Worked Solution: . . . . .	3
1.2	<u>Problem 2</u> . . . . .	4

# Problem Catalogue

Zain Sikand

November 27, 2025

## 1 Integrals: Evil

### 1.1 Problem One

**Problem Author: Zain Sikand**

*Your final answer should be a single expression in the form  $I_1 = [h(x)]_a^b$  where  $b$  and  $a$  are bounds of  $I_1$  to be found*

Conclude whether or not the below integral,  $I_1$  :

$$I_1 = \int_{\int_x^{2x} (\ln x)^2}^{(3+x)^6} \left( \frac{1}{3e^x \cos x \sec^2 x} + \cot x \csc x \right) dx$$

can be written as a single expression, with all integration expressions evaluated.

Your conclusion must be supported, **either**, by an attempt to evaluate the integral or, a proof that  $I_1$  has no real anti-derivative.

—12 Marks—

### 1.1.1 Worked Solution:

$$I_1 = \int_{f_x^{2x}(\ln x)^2}^{(3+x)^6} \left( \frac{1}{3e^x \cos x \sec^2 x} + \cot x \csc x \right) dx$$

$$\Rightarrow I_1 = \int_b^a f(x) dx$$

$\therefore$  let  $I_2 = b$

$$I_2 = \int_x^{2x} (\ln |x|)^2 = \int_{e^u}^{2e^u} u^2 e^u du = [u^2 e^u]_{e^u}^{2e^u} - \int_{e^u}^{2e^u} 2ue^u e^u du$$

$$= [u^2 e^u]_{e^u}^{2e^u} - ([2ue^u]_{e^u}^{2e^u} - \int_{e^u}^{2e^u} 2e^u du) = [u^2 e^u]_{e^u}^{2e^u} - [2ue^u - 2e^u]_{e^u}^{2e^u} = [u^2 e^u - 2ue^u + 2e^u]_{e^u}^{2e^u}$$

$$= [x(\ln |x|)^2 - 2x \ln |x| + 2x]_x^{2x} \because u = \ln |x| \Rightarrow e^u = x$$

$$\therefore I_2 = x[2(\ln |2x|)^2 - (\ln |x|)^2 - \ln |16x^2|]$$

This result can be obtained by evaluating the bounds

$$I_1 = \int_{I_2}^{(3+x)^6} \left( \frac{1}{3e^x \cos x \sec^2 x} + \cot x \csc x \right) dx = \int_a^b \left( \frac{1}{3e^x \cos x \sec^2 x} \right) + \int_a^b \cot x \csc x$$

$$\text{let } I_3 = \int_a^b \left( \frac{1}{3e^x \cos x \sec^2 x} \right) = \int_a^b \left( \frac{1}{3e^x \sec x} \right) dx = \frac{1}{3} \int_a^b (e^{-x} \cos x) dx$$

$$I_3 = 1/3(J)$$

$$J = [-e^{-x} \cos x]_a^b - \int_a^b -e^{-x} \sin x = [-e^{-x} \cos x]_a^b - ([-e^{-x} \sin x]_a^b - \int_a^b e^{-x} \cos x)$$

$$J = [-e^{-x} \cos x]_a^b - [e^{-x} \sin x]_a^b - J$$

$$\therefore J = \frac{1}{2} [e^{-x} \sin x - e^{-x} \cos x]_a^b$$

$$\therefore I_3 = \frac{1}{6} [e^{-x} \sin x - e^{-x} \cos x]_a^b$$

$$I_1 = I_3 + \int_a^b \cot x \csc x dx$$

$$\text{let } I_4 = \int_a^b \cot x \csc x dx$$

$$I_4 = \int_a^b \left( \frac{1}{\sin x} \right) \left( \frac{\cos x}{\sin x} \right) dx = \int_a^b \frac{\cos x}{1 - \cos^2 x} dx$$

**Integrate  $I_4$  by parts:**

$$I_4 = \int_a^b \frac{\cos x}{\sin^2 x} dx = \int_a^b \cos x \left( \frac{1}{\sin^2 x} \right) dx = \left[ \frac{1}{\sin x} \right]_a^b - \int_a^b \sin x \left( \frac{-2 \sin x \cos x}{\sin^4 x} \right) dx = \left[ \frac{1}{\sin x} \right]_a^b - \int_a^b \frac{-2 \cos x}{\sin x} dx$$

$$\therefore I_4 = \left[ \frac{1}{\sin x} \right]_a^b + 2I_4$$

$$\Rightarrow I_4 = -\frac{1}{\sin x}$$

$$\therefore I_1 = [I_3 + I_4]_a^b$$

<sup>1</sup>  $\therefore$  The integral  $I_1$  can be written as a single expression within its bounds  $\therefore$  Q.E.D

## 1.2 Problem 2

---

<sup>1</sup> **Warning:** Solution is unverified